typing.v
@@ -1,105 +1,107 @@
 From WR Require Import imports join common.
 
+Reserved Notation "Γ ⊢ a ∈ A" (at level 70).
+Reserved Notation "⊢ Γ" (at level 70).
+
 Inductive Wt (Γ : context) : tm -> tm -> Prop :=
 | T_Var i :
-  Wff Γ ->
+  ⊢ Γ ->
   i < length Γ ->
   (* ------ *)
-  Wt Γ (var_tm i) (dep_ith Γ i)
+  Γ ⊢ (var_tm i) ∈ (dep_ith Γ i)
 
 | T_Void i :
-  Wff Γ ->
+  ⊢ Γ ->
   (* -------- *)
-  Wt Γ tVoid (tUniv i)
+  Γ ⊢ tVoid ∈ (tUniv i)
 
 | T_Pi i A B :
-  Wt Γ A (tUniv i) ->
-  Wt (A :: Γ) B (tUniv i) ->
+  Γ ⊢ A ∈(tUniv i) ->
+  (A :: Γ) ⊢ B ∈ (tUniv i) ->
   (* --------------------- *)
-  Wt Γ (tPi A B) (tUniv i)
+  Γ ⊢ (tPi A B) ∈ (tUniv i)
 
 | T_Abs A a B i :
-  Wt Γ (tPi A B) (tUniv i) ->
-  Wt (A :: Γ) a B ->
+  Γ ⊢ (tPi A B) ∈ (tUniv i) ->
+  (A :: Γ) ⊢ a ∈ B ->
   (* -------------------- *)
-  Wt Γ (tAbs a) (tPi A B)
+  Γ ⊢ (tAbs a) ∈ (tPi A B)
 
 | T_App a A B b :
-  Wt Γ a (tPi A B) ->
-  Wt Γ b A ->
+  Γ ⊢ a ∈ (tPi A B) ->
+  Γ ⊢ b ∈ A ->
   (* -------------------- *)
-  Wt Γ (tApp a b) (B [ b.. ])
+  Γ ⊢ (tApp a b) ∈ (B [ b.. ])
 
 | T_Conv a A B i :
-  Wt Γ a A ->
-  Wt Γ B (tUniv i) ->
+  Γ ⊢ a ∈ A ->
+  Γ ⊢ B ∈ (tUniv i) ->
   Coherent A B ->
   (* ----------- *)
-  Wt Γ a B
+  Γ ⊢ a ∈ B
 
 | T_True :
-  Wff Γ ->
+  ⊢ Γ ->
   (* --------- *)
-  Wt Γ tTrue tBool
+  Γ ⊢ tTrue ∈ tBool
 
 | T_False :
-  Wff Γ ->
+  ⊢ Γ ->
   (* --------- *)
-  Wt Γ tFalse tBool
+  Γ ⊢ tFalse ∈ tBool
 
 | T_If a b c A i :
-  Wt (tBool :: Γ) A (tUniv i) ->
-  Wt Γ a tBool ->
-  Wt Γ b (A [tTrue..]) ->
-  Wt Γ c (A [tFalse..]) ->
+  (tBool :: Γ) ⊢ A ∈ (tUniv i) ->
+  Γ ⊢ a ∈ tBool ->
+  Γ ⊢ b ∈ (A [tTrue..]) ->
+  Γ ⊢ c ∈ (A [tFalse..]) ->
   (* ------------ *)
-  Wt Γ (tIf a b c) (A [a..])
+  Γ ⊢ (tIf a b c) ∈ (A [a..])
 
 | T_Bool i :
-  Wff Γ ->
+  ⊢ Γ ->
   (* ----------- *)
-  Wt Γ tBool (tUniv i)
+  Γ ⊢ tBool ∈ (tUniv i)
 
 | T_Univ i :
-  Wff Γ ->
+  ⊢ Γ ->
   (* ------------ *)
-  Wt Γ (tUniv i) (tUniv (S i))
+  Γ ⊢ (tUniv i) ∈ (tUniv (S i))
 
 | T_Refl a A:
-  Wff Γ ->
-  Wt Γ a A ->
+  ⊢ Γ ->
+  Γ ⊢ a ∈ A ->
   (* ------ *)
-  Wt Γ tRefl (tEq a a A)
+  Γ ⊢ tRefl ∈ (tEq a a A)
 
 | T_Eq a b A i j :
-  Wt Γ a A ->
-  Wt Γ b A ->
-  Wt Γ A (tUniv j) ->
+  Γ ⊢ a ∈ A ->
+  Γ ⊢ b ∈ A ->
+  Γ ⊢ A ∈ (tUniv j) ->
   (* ----------------------- *)
-  Wt Γ (tEq a b A) (tUniv i)
+  Γ ⊢ (tEq a b A) ∈ (tUniv i)
 
 | T_J t a b p A i j C : 
-  Wt Γ a A ->
-  Wt Γ b A ->
-  Wt Γ A (tUniv j) ->
-  Wt Γ p (tEq a b A) ->
-  Wt (tEq (ren_tm shift a) (var_tm 0) (ren_tm shift A) :: A :: Γ) C (tUniv i) ->
-  Wt Γ t (C [tRefl .: a ..]) ->
-  Wt Γ (tJ t a b p) (C [p .: b..])
-  
-
+  Γ ⊢ a ∈  A ->
+  Γ ⊢ b ∈ A ->
+  Γ ⊢ A ∈ (tUniv j) ->
+  Γ ⊢ p ∈ (tEq a b A) ->
+  (tEq (ren_tm shift a) (var_tm 0) (ren_tm shift A) :: A :: Γ) ⊢ C ∈ (tUniv i) ->
+  Γ ⊢ t ∈ (C [tRefl .: a ..]) ->
+  Γ ⊢ (tJ t a b p) ∈ (C [p .: b..])
 
 with Wff (Γ : context) : Prop :=
 | Wff_intro F :
-  (forall i, i < length Γ -> Wt (skipn (S i) Γ) (ith Γ i) (tUniv (F i))) ->
+  (forall i, i < length Γ -> (skipn (S i) Γ) ⊢ (ith Γ i) ∈ (tUniv (F i))) ->
   (* ---------------------------------------------------------------- *)
-  Wff Γ.
+  ⊢ Γ
+where 
+  "Γ ⊢ a ∈ A" := (Wt Γ a A) and "⊢ Γ" := (Wff Γ).
+
 
 Scheme wt_ind := Induction for Wt Sort Prop
     with wff_ind := Induction for Wff Sort Prop.
 
 Combined Scheme wt_mutual from wt_ind, wff_ind.
 
-(* TODO: use notations in rules *)
-Notation "Γ ⊢ a ∈ A" := (Wt Γ a A) (at level 70).
-Notation "⊢ Γ" := (Wff Γ) (at level 70).
+
